fix spec

specs/experimental/Spec.RSA.Bignum.fst
@@ -30,41 +30,39 @@ type sign =
 val abs_sub: 
     x:size_nat -> a:bignum -> b:bignum -> Pure (tuple2 sign bignum)
     (requires (a < pow2 (pow2 x) /\ b < pow2 (pow2 x)))
-    (ensures (fun (s, res) -> res < pow2 (pow2 x) /\ res = abs (a - b)))
+    (ensures (fun (s, res) -> res < pow2 (pow2 x) /\ res = abs (a - b) /\
+			    s = (if a >= b then Positive else Negative)))
     
 let abs_sub x a b =
     if (bn_is_less a b)
-    then begin
-        assert (b > a);
-        (Negative, b - a) end
-    else begin
-        assert (a >= b);
-        (Positive, a - b) end
+    then (Negative, b - a)
+    else (Positive, a - b)
 
 val add_sign:
     c0:bignum -> c1:bignum -> c2:bignum ->
     a0:bignum -> a1:bignum -> a2:bignum ->
-    b0:bignum -> b1:bignum -> b2:bignum -> Pure bignum
+    b0:bignum -> b1:bignum -> b2:bignum ->
+    sa2:sign -> sb2:sign -> Pure bignum
     (requires (c0 == a0 * b0 /\ c1 == a1 * b1 /\ c2 == a2 * b2 /\
-               a2 = abs (a0 - a1) /\ b2 = abs (b0 - b1)))
+               a2 = abs (a0 - a1) /\ b2 = abs (b0 - b1) /\
+	       sa2 = (if (a0 >= a1) then Positive else Negative) /\
+	       sb2 = (if (b0 >= b1) then Positive else Negative)))
     (ensures (fun res -> res == a1 * b0 + a0 * b1))
 
 #reset-options "--z3rlimit 150 --initial_fuel 0 --max_fuel 0"
 
-let add_sign c0 c1 c2 a0 a1 a2 b0 b1 b2 =
-    let sa2 = if (a0 >= a1) then Positive else Negative in
-    let sb2 = if (b0 >= b1) then Positive else Negative in
-    if ((sa2 = Positive && sb2 = Positive) || (sa2 = Negative && sb2 = Negative)) 
+let add_sign c0 c1 c2 a0 a1 a2 b0 b1 b2 sa2 sb2 =
+    if ((sa2 = Positive && sb2 = Positive) || (sa2 = Negative && sb2 = Negative))
     then (c0 + c1) - c2
     else (c0 + c1) + c2
 
 val karatsuba:
-    x0:size_nat -> a:bignum{a < pow2 (pow2 x0)} -> b:bignum{b < pow2 (pow2 x0)} -> Pure bignum
+    x0:size_nat{0 < x0} -> a:bignum{a < pow2 (pow2 x0)} -> b:bignum{b < pow2 (pow2 x0)} -> Pure bignum
     (requires (True))
     (ensures (fun res -> res == a * b))
     (decreases x0)
 
-#reset-options "--z3rlimit 150 --max_fuel 2"
+#reset-options "--z3rlimit 300 --max_fuel 2"
 
 let rec karatsuba x0 a b =
     if x0 < 9 then a * b
@@ -95,7 +93,7 @@ let rec karatsuba x0 a b =
         assert (c2 == a2 * b2); //from ind hypo
 		
         let pow_x1 = pow2 (pow2 (x + 1)) in
-        let tmp = add_sign c0 c1 c2 a0 a1 a2 b0 b1 b2 in
+        let tmp = add_sign c0 c1 c2 a0 a1 a2 b0 b1 b2 sa2 sb2 in
         let c = c1 * pow_x1 + tmp * pow_x + c0 in
         lemma_karatsuba_mult x a a0 a1 b b0 b1;
         assert (c == a * b);
@@ -103,14 +101,14 @@ let rec karatsuba x0 a b =
     end
 
 val mont_reduction:
-    modBits:size_nat{1 < modBits /\ modBits < pow2 32} ->
-    r:nat{r = pow2 (modBits + 2) /\ r > 0} ->
+    modBits:size_nat{1 < modBits} ->
+    r:nat{r = pow2 (modBits + 2) /\ 0 < r} ->
     n:nat{1 < n /\ 4 * n < r} -> n':bignum ->
     c:nat{c < r * n} -> Pure (elem (n + n))
     (requires (True))
     (ensures (fun res -> res % n == (c / r) % n))
 
-#reset-options "--z3rlimit 300 --max_fuel 0"
+#reset-options "--z3rlimit 150 --max_fuel 0"
 
 let mont_reduction modBits r n n' c =
     let m = (c * n') % r in
@@ -124,58 +122,65 @@ let mont_reduction modBits r n n' c =
     assert (res <= (c + n * r) / r);
     division_addition_lemma c r n;
     assert (res <= c / r + n);
-    assert (c / r < n);
+    assert (c < r * n);
+    division_addition_lemma 0 r n;
     assert (res < n + n);
     lemma_mont_reduction res r c n m;
     res
 
 val mul_mod_mont:
     x0:size_nat ->
-    modBits:size_nat{1 < modBits /\ modBits < pow2 32} ->
-    r:nat{r = pow2 (modBits + 2) /\ r > 0} ->
+    modBits:size_nat{1 < modBits} ->
+    r:nat{r = pow2 (modBits + 2) /\ 0 < r} ->
     n:nat{1 < n /\ 4 * n < r /\ r <= pow2 (pow2 x0)} -> n':bignum ->
     a:elem (n + n) -> b:elem (n + n) -> Pure (elem (n + n))
     (requires (True))
     (ensures (fun res -> res % n == (a * b / r) % n))
-    
+
+#reset-options "--z3rlimit 50 --max_fuel 0"
+
 let mul_mod_mont x0 modBits r n n' a b =
-    let c = karatsuba x0 a b in
+    //let c = karatsuba x0 a b in
+    let c = a * b in
     assert (c < 4 * n * n);
-    assert (c < r * n);
+    //assert (c < r * n);
     mont_reduction modBits r n n' c
 
 val to_mont:
-    modBits:size_nat{1 < modBits /\ modBits < pow2 32} ->
-    r:nat{r = pow2 (modBits + 2) /\ r > 0} ->
+    modBits:size_nat{1 < modBits} ->
+    r:nat{r = pow2 (modBits + 2) /\ 0 < r} ->
     n:nat{1 < n /\ 4 * n < r} -> n':bignum ->
     r2:elem n -> a:elem n -> Pure (elem (n + n))
     (requires (r2 == (r * r) % n))
     (ensures (fun res -> res % n == (a * r) % n))
-    
+
+#reset-options "--z3rlimit 150 --max_fuel 0"
+
 let to_mont modBits r n n' r2 a =
     let c = a * r2 in
     assert (c == a * ((r * r) % n));
-    assert (c < n * n);
-    assert (c < r * n);
+    assert (c < 4 * n * n);
     let res = mont_reduction modBits r n n' c in
     assert (res % n == ((a * ((r * r) % n)) / r) % n);
     lemma_mod_div_simplify res a r n;
     res
 
 val from_mont:
-    modBits:size_nat{1 < modBits /\ modBits < pow2 32} ->
-    r:nat{r = pow2 (modBits + 2) /\ r > 0} ->
+    modBits:size_nat{1 < modBits} ->
+    r:nat{r = pow2 (modBits + 2) /\ 0 < r} ->
     n:nat{1 < n /\ 4 * n < r} -> n':bignum ->
     a_r:elem (n + n) -> Pure (elem n)
     (requires (True))
     (ensures (fun res -> res == (a_r / r) % n))
-    
+
+#reset-options "--z3rlimit 150 --max_fuel 0"
+
 let from_mont modBits r n n' a_r =
     let m = (a_r * n') % r in
     assert (0 <= m /\ m < r);
     let m = r - m in
     assert (0 < m /\ m <= r);
-    let res:nat = (a_r + n * m) / r in
+    let res = (a_r + n * m) / r in
     assert (a_r + n * m <= a_r + n * r);
     lemma_div_le (a_r + n * m) (a_r + n * r) r;
     assert (res <= (a_r + n * r) / r);
@@ -193,15 +198,18 @@ val degree_: a:bignum -> i:size_nat -> Tot size_nat (decreases i)
 let rec degree_ a i =
   if i = 0 then 0
   else
-    if is_bit_set a i then i
-    else degree_ a (i-1)
+    if is_bit_set a (i - 1) then i
+    else degree_ a (i - 1)
 
+val degree: a:bignum -> aBits:size_nat -> Tot size_nat
 let degree a aBits = degree_ a aBits
 
-val bn_shift_left: a:bignum -> b:size_nat -> Tot bignum
-let bn_shift_left a b = a * pow2 b
+val bn_lshift: a:bignum -> b:size_nat -> Tot bignum
+let bn_lshift a b = a * pow2 b
 
-val shift_euclidean_mod_inv_f: m:bignum -> tmp:bignum -> f:size_nat -> i:size_nat -> Tot bignum
+val shift_euclidean_mod_inv_f:
+    m:bignum -> tmp:bignum{tmp <= m} -> f:size_nat -> i:size_nat -> Tot (res:bignum{res <= m}) 
+    (decreases (f - i))
 let rec shift_euclidean_mod_inv_f m tmp f i =
     if (i < f) then begin
       let tmp = tmp + tmp in
@@ -210,33 +218,47 @@ let rec shift_euclidean_mod_inv_f m tmp f i =
     else tmp
 
 // u >= v
-val shift_euclidean_mod_inv_: 
-    uBits:size_nat -> u:bignum -> vBits:size_nat{uBits > vBits} -> v:bignum -> r:bignum -> s:bignum -> m:bignum -> Tot bignum
-let rec shift_euclidean_mod_inv_ uBits u vBits v r s m =
-    let du = degree u uBits in
-    let dv = degree v vBits in
-   
-    if dv > 0 then begin
-      let f = du - dv in //u >= v
-      let v_lshift_f = bn_shift_left v f in
-      let f = if (u < v_lshift_f) then f - 1 else f in
-      let v_lshift_f = bn_shift_left v f in
-      let u = u - v_lshift_f in
+val shift_euclidean_mod_inv_:
+    du:size_nat -> u:bignum -> dv:size_nat{dv <= du} -> v:bignum{v <= u} ->
+    r:bignum -> s:bignum -> m:bignum{s < m /\ r < m} -> Tot bignum
+    (decreases (du + dv))
     
-      let tmp = shift_euclidean_mod_inv_f m s f 0 in
+let rec shift_euclidean_mod_inv_ du u dv v r s m =
+    if dv > 1 then begin
+      let f = du - dv in
+      let (u, f) =
+         if (f > 0) then begin
+            let v_lshift_f = bn_lshift v f in
+            let f = if (u < v_lshift_f) then f - 1 else f in
+            let v_lshift_f = bn_lshift v f in
+            assume (0 <= u - v_lshift_f);
+            let u = u - v_lshift_f in
+            (u, f) end
+          else (u - v, f) in
+	 
+      let tmp = if (f > 0) then shift_euclidean_mod_inv_f m s f 0 else s in
+      assert (tmp <= m);
       let r = if (r < tmp) then r + m - tmp else r - tmp in
-      let du = degree u uBits in
-      if (u < v) then
+      assume (r < m);
+
+      let du' = degree u du in
+      assume (du' < du);
+      if (u < v) then begin
         //swap (u, v); swap (r, s)
-        shift_euclidean_mod_inv_ dv v du u s r m
-      else shift_euclidean_mod_inv_ du u dv v r s m end
+	assume (du' <= dv);
+        shift_euclidean_mod_inv_ dv v du' u s r m end
+      else begin
+        assume (dv <= du');
+        shift_euclidean_mod_inv_ du' u dv v r s m end
+    end
     else s
           
 //res = a^(-1) % m
-val shift_euclidean_mod_inv: aBits:size_nat ->a:bignum -> mBits:size_nat -> m:bignum -> Tot bignum
+val shift_euclidean_mod_inv:
+    aBits:size_nat -> a:bignum -> 
+    mBits:size_nat{aBits < mBits} -> m:bignum{1 < m /\ a < m} -> Tot bignum
 let shift_euclidean_mod_inv aBits a mBits m =
-    //a < m
-    let r = 0 in 
+    let r = 0 in
     let s = 1 in
     shift_euclidean_mod_inv_ mBits m aBits a r s m
 
@@ -298,6 +320,25 @@ let mod_exp x0 modBits n a b =
     lemma_mod_mult_div_1 ((pow a b) * r) r n;
     multiple_division_lemma (pow a b) r;
     res
+
+val rsa_blinding:
+    x0:size_nat ->
+    modBits:size_nat{1 < modBits /\ modBits + 3 < pow2 32} ->
+    n:bignum{1 < n /\ n < pow2 modBits /\ pow2 (modBits + 2) < pow2 (pow2 x0)} ->
+    p:elem n{1 < p} ->
+    q:elem n{1 < q /\ n = p * q} ->
+    d:elem n{1 < d} ->
+    m:elem n ->
+    rBlind:bignum{rBlind < pow2 64} -> Tot (s:bignum{s == (pow m d) % n})
+
+let rsa_blinding x0 modBits n p q d m rBlind =
+    let phi_n:nat = (p - 1) * (q - 1) in
+    let d':nat = d + rBlind * phi_n in
+    let s = mod_exp x0 modBits n m d' in
+    assert (s == (pow m d') % n);
+    lemma_exp_blinding n phi_n p q d m rBlind;
+    assert (s == (pow m d) % n);
+    s
 
 (* BIGNUM CONVERT FUNCTIONS *)
 val os2ip:bLen:size_nat{bLen > 0} -> b:lbytes bLen -> Tot (res:bignum{res < pow2 (8 * bLen)})
