specs/experimental/Spec.RSA.fst
@@ -96,6 +96,7 @@ let pss_encode_ sLen salt msgLen msg emLen em =
     let mHash = create hLen (u8 0) in
     let mHash = hash_sha256 msgLen msg mHash in
 
+    //m1 = [8 * 0x00; mHash; salt]
     let m1_size : size_nat = 8 + hLen + sLen in
     let m1 = create m1_size (u8 0) in
     let m1 = update_sub m1 8 hLen mHash in
@@ -105,6 +106,7 @@ let pss_encode_ sLen salt msgLen msg emLen em =
     let m1Hash' = hash_sha256 m1_size m1 m1Hash' in
     let m1Hash = update_sub m1Hash 0 hLen m1Hash' in
 
+    //db = [0x00; ..; 0x00; 0x01; salt]
     let db_size : size_nat = emLen - hLen - 1 in
     let db = create db_size (u8 0) in
     let last_before_salt = db_size - sLen - 1 in
@@ -114,9 +116,10 @@ let pss_encode_ sLen salt msgLen msg emLen em =
     let dbMask = create db_size (u8 0) in
     let dbMask = mgf_sha256 (hLen + 4) m1Hash db_size dbMask in
     let maskedDB = xor_bytes db_size db dbMask in
+    //em = [maskedDB; m1Hash'; 0xbc]
     let em = update_sub em 0 db_size maskedDB in
     let em = update_sub em db_size hLen m1Hash' in
-    em.[emLen - 1] <- (u8 188)
+    em.[emLen - 1] <- (u8 0xbc)
 
 val pss_encode:
     msBits:size_nat{msBits < 8} ->
@@ -137,7 +140,7 @@ let pss_encode msBits sLen salt msgLen msg emLen em =
     else begin
         let em = pss_encode_ sLen salt msgLen msg emLen em in
         assert (0 < 8 - msBits /\ 8 - msBits < 8);
-        em.[0] <- em.[0] &. ((u8 255) >>. u32 (8 - msBits)) end
+        em.[0] <- em.[0] &. ((u8 0xff) >>. u32 (8 - msBits)) end
 
 val pss_verify_:
     sLen:size_nat{sLen + hLen + 8 < pow2 32 /\ sLen + hLen + 8 < max_input_len_sha256} ->
@@ -153,7 +156,7 @@ let pss_verify_ sLen msBits emLen em msgLen msg =
 
     let (pad_size:size_nat{pad_size > 0}) = emLen - sLen - hLen - 1 in
     let pad2 = create pad_size (u8 0) in
-    let pad2 = pad2.[pad_size - 1] <- (u8 1) in
+    let pad2 = pad2.[pad_size - 1] <- (u8 0x01) in
 
     let (db_size:size_nat{db_size > 0}) = emLen - hLen - 1 in
     let maskedDB = slice em 0 db_size in
@@ -167,7 +170,7 @@ let pss_verify_ sLen msBits emLen em msgLen msg =
         if msBits > 0
         then begin
             assert (0 < 8 - msBits /\ 8 - msBits < 8);
-            db.[0] <- db.[0] &. (u8 255 >>. u32 (8 - msBits)) end
+            db.[0] <- db.[0] &. (u8 0xff >>. u32 (8 - msBits)) end
         else db in
 	
     let pad = slice db 0 pad_size in
@@ -194,10 +197,10 @@ val pss_verify:
     msg:lbytes msgLen -> Tot bool
 
 let pss_verify sLen msBits emLen em msgLen msg =
-    let em_0 = em.[0] &. (u8 255 <<. u32 msBits) in
+    let em_0 = em.[0] &. (u8 0xff <<. u32 msBits) in
     let em_last = em.[emLen - 1] in
 
-    if not ((uint_to_nat #U8 em_0 = 0) && (uint_to_nat #U8 em_last = 188))
+    if not ((uint_to_nat #U8 em_0 = 0) && (uint_to_nat #U8 em_last = 0xbc))
     then false
     else begin
         let emLen' = if msBits = 0 then emLen - 1 else emLen in
@@ -206,25 +209,6 @@ let pss_verify sLen msBits emLen em msgLen msg =
         then false
         else pss_verify_ sLen msBits emLen' em' msgLen msg
     end
-
-val rsa_blinding:
-    x0:size_nat ->
-    modBits:modBits ->
-    n:bignum{1 < n /\ n < pow2 modBits /\ pow2 (modBits + 2) < pow2 (pow2 x0)} ->
-    p:elem n{1 < p} ->
-    q:elem n{1 < q /\ n = p * q} ->
-    d:elem n{1 < d} ->
-    m:elem n ->
-    rBlind:bignum{rBlind < pow2 64} -> Tot (s:bignum{s == (pow m d) % n})
-
-let rsa_blinding x0 modBits n p q d m rBlind =
-    let phi_n:nat = (p - 1) * (q - 1) in
-    let d':nat = d + rBlind * phi_n in
-    let s = mod_exp x0 modBits n m d' in
-    assert (s == (pow m d') % n);
-    lemma_exp_blinding n phi_n p q d m rBlind;
-    assert (s == (pow m d) % n);
-    s
 
 val rsa_sign:
     x0:size_nat ->
